Weidenbach_Book/IsaSAT_Restart.thy
@@ -302,4 +302,136 @@ lemma (in -) isasat_fast_alt_def:
   unfolding isasat_fast_def
   by (auto intro!:ext)
 
+definition cdcl_twl_stgy_restart_prog_bounded_wl_heur
+   :: "twl_st_wl_heur \<Rightarrow> (bool \<times> twl_st_wl_heur) nres"
+where
+  \<open>cdcl_twl_stgy_restart_prog_bounded_wl_heur S\<^sub>0 = do {
+    ebrk \<leftarrow> RETURN (\<not>isasat_fast S\<^sub>0);
+    (ebrk, brk, T, n) \<leftarrow>
+     WHILE\<^sub>T\<^bsup>\<lambda>(ebrk, brk, T, n). cdcl_twl_stgy_restart_abs_wl_heur_inv S\<^sub>0 brk T n \<and>
+        (\<not>ebrk \<longrightarrow>isasat_fast T) \<and> length (get_clauses_wl_heur T) \<le> uint64_max\<^esup>
+      (\<lambda>(ebrk, brk, _). \<not>brk \<and> \<not>ebrk)
+      (\<lambda>(ebrk, brk, S, n).
+      do {
+        ASSERT(\<not>brk \<and> \<not>ebrk);
+        ASSERT(length (get_clauses_wl_heur S) \<le> uint64_max);
+        T \<leftarrow> unit_propagation_outer_loop_wl_D_heur S;
+        ASSERT(length (get_clauses_wl_heur T) \<le> uint64_max);
+        ASSERT(length (get_clauses_wl_heur T) = length (get_clauses_wl_heur S));
+        (brk, T) \<leftarrow> cdcl_twl_o_prog_wl_D_heur T;
+        ASSERT(length (get_clauses_wl_heur T) \<le> uint64_max);
+        (T, n) \<leftarrow> restart_prog_wl_D_heur T n brk;
+	ebrk \<leftarrow> RETURN (\<not>isasat_fast T);
+        RETURN (ebrk, brk, T, n)
+      })
+      (ebrk, False, S\<^sub>0::twl_st_wl_heur, 0);
+    RETURN (brk, T)
+  }\<close>
+
+
+lemma cdcl_twl_stgy_restart_prog_bounded_wl_heur_cdcl_twl_stgy_restart_prog_bounded_wl_D:
+  assumes r: \<open>r \<le> uint64_max\<close>
+  shows \<open>(cdcl_twl_stgy_restart_prog_bounded_wl_heur, cdcl_twl_stgy_restart_prog_bounded_wl_D) \<in>
+   twl_st_heur''' r \<rightarrow>\<^sub>f \<langle>bool_rel \<times>\<^sub>r twl_st_heur\<rangle>nres_rel\<close>
+proof -
+  have cdcl_twl_stgy_restart_prog_bounded_wl_D_alt_def:
+  \<open>cdcl_twl_stgy_restart_prog_bounded_wl_D S\<^sub>0 = do {
+      ebrk \<leftarrow> RES UNIV;
+      (ebrk, brk, T, n) \<leftarrow> WHILE\<^sub>T\<^bsup>\<lambda>(_, brk, T, n). cdcl_twl_stgy_restart_abs_wl_D_inv S\<^sub>0 brk T n\<^esup>
+	        (\<lambda>(ebrk, brk, _). \<not>brk \<and> \<not>ebrk)
+	        (\<lambda>(_, brk, S, n).
+	        do {
+	          T \<leftarrow> unit_propagation_outer_loop_wl_D S;
+	          (brk, T) \<leftarrow> cdcl_twl_o_prog_wl_D T;
+	          (T, n) \<leftarrow> restart_prog_wl_D T n brk;
+	          ebrk \<leftarrow> RES UNIV;
+	          RETURN (ebrk, brk, T, n)
+	        })
+	        (ebrk, False, S\<^sub>0::nat twl_st_wl, 0);
+      RETURN (brk, T)
+    }\<close> for S\<^sub>0
+    unfolding cdcl_twl_stgy_restart_prog_bounded_wl_D_def nres_monad1 by auto
+  have [refine0]: \<open>RETURN (\<not>isasat_fast x) \<le> \<Down>
+      {(b, b'). b = b' \<and> (b = (\<not>isasat_fast x))} (RES UNIV)\<close>
+    for x
+    by (auto intro: RETURN_RES_refine)
+  have [refine0]: \<open>isasat_fast_slow x1e
+      \<le> \<Down> {(S, S'). S = x1e \<and> S' = x1b}
+	   (RETURN x1b)\<close>
+    for x1e x1b
+  proof -
+    show ?thesis
+      unfolding isasat_fast_slow_alt_def by auto
+  qed
+  have twl_st_heur'': \<open>(x1e, x1b) \<in> twl_st_heur \<Longrightarrow>
+    (x1e, x1b)
+    \<in> twl_st_heur''
+        (dom_m (get_clauses_wl x1b))
+        (length (get_clauses_wl_heur x1e))\<close>
+    for x1e x1b
+    by (auto simp: twl_st_heur'_def)
+  have twl_st_heur''': \<open>(x1e, x1b) \<in> twl_st_heur'' \<D> r \<Longrightarrow>
+    (x1e, x1b)
+    \<in> twl_st_heur''' r\<close>
+    for x1e x1b r \<D>
+    by (auto simp: twl_st_heur'_def)
+  have H: \<open>(xb, x'a)
+    \<in> bool_rel \<times>\<^sub>f
+      twl_st_heur'''' (length (get_clauses_wl_heur x1e) + 6 + uint_max div 2) \<Longrightarrow>
+    x'a = (x1f, x2f) \<Longrightarrow>
+    xb = (x1g, x2g) \<Longrightarrow>
+    (x1g, x1f) \<in> bool_rel \<Longrightarrow>
+    (x2e, x2b) \<in> nat_rel \<Longrightarrow>
+    (((x2g, x2e), x1g), (x2f, x2b), x1f)
+    \<in> twl_st_heur''' (length (get_clauses_wl_heur x2g)) \<times>\<^sub>f
+      nat_rel \<times>\<^sub>f
+      bool_rel\<close> for x y ebrk ebrka xa x' x1 x2 x1a x2a x1b x2b x1c x2c x1d x2d x1e x2e T Ta xb
+       x'a x1f x2f x1g x2g
+    by auto
+  have abs_inv: \<open>(x, y) \<in> twl_st_heur''' r \<Longrightarrow>
+    (ebrk, ebrka) \<in> {(b, b'). b = b' \<and> b = (\<not> isasat_fast x)} \<Longrightarrow>
+    (xb, x'a) \<in> bool_rel \<times>\<^sub>f (twl_st_heur \<times>\<^sub>f nat_rel) \<Longrightarrow>
+    case x'a of
+    (brk, xa, xb) \<Rightarrow>
+      cdcl_twl_stgy_restart_abs_wl_D_inv y brk xa xb \<Longrightarrow>
+    x2f = (x1g, x2g) \<Longrightarrow>
+    xb = (x1f, x2f) \<Longrightarrow>
+    cdcl_twl_stgy_restart_abs_wl_heur_inv x x1f x1g x2g\<close>
+   for x y ebrk ebrka xa x' x1 x2 x1a x2a x1b x2b x1c x2c x1d x2d
+       x1e x2e T Ta xb x'a x1f x2f x1g x2g
+    unfolding cdcl_twl_stgy_restart_abs_wl_heur_inv_def by fastforce
+  show ?thesis
+    supply[[goals_limit=1]] isasat_fast_length_leD[dest] twl_st_heur'_def[simp]
+    unfolding cdcl_twl_stgy_restart_prog_bounded_wl_heur_def
+      cdcl_twl_stgy_restart_prog_bounded_wl_D_alt_def
+    apply (intro frefI nres_relI)
+    apply (refine_rcg
+        restart_prog_wl_D_heur_restart_prog_wl_D[THEN fref_to_Down_curry2]
+        cdcl_twl_o_prog_wl_D_heur_cdcl_twl_o_prog_wl_D[THEN fref_to_Down]
+        unit_propagation_outer_loop_wl_D_heur_unit_propagation_outer_loop_wl_D'[THEN fref_to_Down]
+        WHILEIT_refine[where R = \<open>{((ebrk, brk, T,n), (ebrk', brk', T', n')).
+	    (ebrk = ebrk') \<and> (brk = brk') \<and> (T, T')  \<in> twl_st_heur \<and> n = n' \<and>
+	      (\<not>ebrk \<longrightarrow> isasat_fast T) \<and> length (get_clauses_wl_heur T) \<le> uint64_max}\<close>])
+    subgoal using r by auto
+    subgoal
+      unfolding cdcl_twl_stgy_restart_abs_wl_heur_inv_def by fast
+    subgoal by auto
+    subgoal by auto
+    subgoal by auto
+    subgoal by auto
+    subgoal by fast
+    subgoal by auto
+    apply (rule twl_st_heur''; auto; fail)
+    subgoal by auto
+    subgoal by auto
+    apply (rule twl_st_heur'''; assumption)
+    subgoal by (auto simp: isasat_fast_def uint64_max_def uint32_max_def)
+    apply (rule H; assumption?)
+    subgoal by auto
+    subgoal by auto
+    subgoal by auto
+    subgoal by auto
+    done
+qed
+
 end
